# Chap 1. Challenging Exercises

:::{exercise} Expand and simplify the following expressions.

1. $(a+b)(a-b)$ 

	```{admonition} Answer
	$(a+b)(a-b)=a^2-b^2$ 
	```

1. $(a+b)^2$
    ```{admonition} Answer
    $(a+b)^2=a^2+2ab+b^2$ 
    ```

1. $(a-b)^2$
    ```{admonition} Answer
    $(a-b)^2=a^2-2ab+b^2$ 
    ```

1. $(a+b)(a^2-ab+b^2)$
    ```{admonition} Answer
    $(a+b)(a^2-ab+b^2)=a^3+b^3$
    ```

1. $(a-b)(a^2+ab+b^2)$
    ```{admonition} Answer
    $(a-b)(a^2+ab+b^2)=a^3-b^3$
    ```

1. $(a+b+c)^2$
    ```{admonition} Answer
    \begin{align*}
    ~&(a+b+c)^2\\
    =&a^2+b^2+c^2+2ab+2bc+2ac
    \end{align*}
    ```

1. $(a+b+c)(a^2+b^2+c^2-ab-bc-ca)$
    ```{admonition} Answer
    \begin{align*}
    ~&(a+b+c)(a^2+b^2+c^2-ab-bc-ca) \\
    =&a^3+b^3+c^3-3abc
    \end{align*}
    ```

1. $(a+b)(m+n)$
    ```{admonition} Answer
    $(a+b)(m+n)=am+an+bm+bn$
    ```
:::


%Q2
:::{exercise}
Suppose $a$, $b$ and $c$ are three sides of a triangle $\triangle{ABC}$, and they satisfy the equation 

$$a^2+b^2+c^2=ab+bc+ca$$ 

What type of the triangle $\triangle{ABC}$ is? 

1. Right-angle triangle
1. Isosceles triangle
1. Equilateral triangle 


```{admonition} Answer
$$
\begin{aligned}
	~ & \quad  a^2+b^2+c^2=ab+bc+ca \\
	\Rightarrow & \quad 2a^2+2b^2+2c^2=2ab+2bc+2ca \\
	\Rightarrow & \quad a^2+b^2-2ab + a^2+c^2-2ca + b^2+c^2-2bc= 0 \\
	\Rightarrow & \quad (a-b)^2+(a-c)^2+(b-c)^2= 0 \\
	\Rightarrow & \quad a=b=c
\end{aligned}
$$

$\therefore \triangle{ABC}$ is an equilateral triangle.
```

:::


%Q3
:::{exercise} Factorise the following expressions.
1. $2ax-10ay+5by-bx$
    ```{admonition} Answer
    \begin{align*}
      ~&2ax-10ay+5by-bx \\
      =&2a(x-5y)-b(x-5y)\\
      =&(2a-b)(x-5y)
    \end{align*}
    ```
  
1. $a^2-ab+ac-bc$
    ```{admonition} Answer
    \begin{align*}
      ~&a^2-ab+ac-bc\\
      =&a(a-b)+c(a-b) \\
      =&(a+c)(a-b)
    \end{align*}
    ```
  
1. $xy-x-y+1$
    ```{admonition} Answer
    \begin{align*}
      ~ & xy-x-y+1 \\
      = & x(y-1)-(y-1)\\
      = &(x-1)(y-1)
    \end{align*}
    ```
  
1. $x^2-y^2+ax+ay$
    ```{admonition} Answer
    \begin{align*}
      ~ & x^2-y^2+ax+ay \\
      = &(x-y)(x+y)+a(x+y) \\
      = &(x+y)(x-y+a)
    \end{align*}
    ```
  
1. $a^2-2ab+b^2-c^2$
    ```{admonition} Answer
    \begin{align*}
      ~ & a^2-2ab+b^2-c^2 \\
      = &(a-b)^2-c^2\\
      = &(a-b+c)(a-b-c)
    \end{align*}
    ```
  
1. $x^2-x-9y^2-3y$
    ```{admonition} Answer
    \begin{align*}
      ~& x^2-x-9y^2-3y\\
      =&(x^2-9y^2)-(x+3y)\\
      =&(x-3y)(x+3y)-(x+3y)\\
      =&(x-3y-1)(x+3y)
    \end{align*}
    ```
  
1. $x^2-y^2-z^2-2yz$
    ```{admonition} Answer
    \begin{align*}
      ~& x^2-y^2-z^2-2yz\\
      = &x^2-(y^2+2yz+z^2)\\
      = &x^2-(y+z)^2\\
      = &(x+y+z)(x-y-z)
    \end{align*}
    ```
  
1. $x^3+x^2y-xy^2-y^3$
    ```{admonition} Answer
    \begin{align*}
      ~& x^3+x^2y-xy^2-y^3\\
      = &x^2(x+y)-y^2(x+y)\\
      = &(x^2-y^2)(x+y)\\
      = &(x-y)(x+y)^2
    \end{align*}
    ```
  
1. $ax^2-bx^2+bx-ax+a-b$
    ```{admonition} Answer
    \begin{align*}
      ~ & ax^2-bx^2+bx-ax+a-b \\
      = &x^2(a-b)-x(a-b)+(a-b)\\
      = &(a-b)(x^2-x+1)
    \end{align*}
    ```
  
1. $x^2+6xy+9y^2-16a^2+8a-1$
    ```{admonition} Answer
    \begin{align*}
      ~ & x^2+6xy+9y^2-16a^2+8a-1 \\
      = &(x+3y)^2-(4a-1)^2\\
      = &(x+3y+4a-1)(x+3y-4a+1)
    \end{align*}
    ```
  
1. $a^2-6ab+12b+9b^2-4a$
    ```{admonition} Answer
    \begin{align*}
      ~& a^2-6ab+12b+9b^2-4a\\
      = &(a^2-6ab+9b^2)-4(a-3b)\\
      = &(a-3b)^2-4(a-3b)\\
      = &(a-3b)(a-3b-4)
    \end{align*}
    ```
  
1. $a^4-2a^3+a^2-9$
    ```{admonition} Answer
    \begin{align*}
      ~& a^4-2a^3+a^2-9\\
      = &(a^2-a)^2-9\\
      = &(a^2-a+3)(a^2-a-3)
    \end{align*}
    ```
  
1. $4a^2x-4a^2y-b^2x+b^2y$
    ```{admonition} Answer
    \begin{align*}
      ~& 4a^2x-4a^2y-b^2x+b^2y \\
      = &4a^2(x-y)-b^2(x-y)\\
      = &(x-y)(2a+b)(2a-b)
    \end{align*}
    ```
  
1. $x^2-2xy-xz+yz+y^2$
    ```{admonition} Answer
    \begin{align*}
      ~& x^2-2xy-xz+yz+y^2 \\
      = &(x-y)^2-z(x-y) \\
      = &(x-y)(x-y-z)
    \end{align*}
    ```
  
1. $a^2-2a+b^2-2b+2ab+1$
    ```{admonition} Answer
    \begin{align*}
      ~& a^2-2a+b^2-2b+2ab+1 \\
      = &a^2+2ab+b^2-2a-2b+1\\
      = &(a+b)^2-2(a+b)+1 \\
      = &(a+b-1)^2
    \end{align*}
    ```
  
1. $(a+c)(a-c)+b(b-2a)$
    ```{admonition} Answer
    \begin{align*}
      ~ & (a+c)(a-c)+b(b-2a)\\
      = &a^2-c^2+b^2-2ab\\
      = &(a^2-2ab+b^2)-c^2\\
      = &(a-b+c)(a-b-c)
    \end{align*}
    ```
:::

%Q4
:::{exercise} Factorise the following expressions.

1. $3x^2-11x+10$
    ```{admonition} Answer    
    $3x^2-11x+10=(3x-5)(x-2)$
    ```
  
1. $15x^2+7xy-4y^2$
    ```{admonition} Answer
    $15x^2+7xy-4y^2=(3x-y)(5x+4y)$
    ```
  
1. $a^2x^2-6ax+8$
    ```{admonition} Answer
    $a^2x^2-6ax+8=(ax-2)(ax-4)$
    ```
  
1. $m^2-4mn+4n^2-3m+6n+2$
    ```{admonition} Answer
    \begin{align*}
      ~& m^2-4mn+4n^2-3m+6n+2\\
      = &(m-2n)^2-3(m-2n)+2\\
      = &(m-2n-1)(m-2n-2)
    \end{align*}		
    ```
  
1. $4x^2-4xy-6x+3y+y^2-10$
    ```{admonition} Answer
    \begin{align*}
      ~&4x^2-4xy-6x+3y+y^2-10 \\
       = &(2x-y)^2-3(2x-y)-10 \\
      = &(2x-y-5)(2x-y+2)
    \end{align*}
    ```
  
1. $12(x+y)^2+11(x^2-y^2)+2(x-y)^2$
    ```{admonition} Answer
    \begin{align*}
     ~& 12(x+y)^2+11(x^2-y^2)+2(x-y)^2 \\
     = &\left[3(x+y)+2(x-y)\right] \left[4(x+y)+(x-y)\right] \\
     = &(5x+y)(5x+3y)
    \end{align*}
    ```
  
1. $abcx^2+(a^2b^2+c^2)x+abc$
    ```{admonition} Answer
    $abcx^2+(a^2b^2+c^2)x+abc=(abx+c)(cx+ab)$
    ```
  
1. $2005x^2-(2005^2-1)x-2005$
    ```{admonition} Answer
    $2005x^2-(2005^2-1)x-2005=(2005x+1)(x-2005)$
    ```
  
1. $(x+1)(x+2)(x+3)(x+6)+x^2$
    ```{admonition} Answer
    \begin{align*}
      ~&(x+1)(x+2)(x+3)(x+6)+x^2 \\
      = &(x^2+7x+6)(x^2+5x+6)+x^2 \\
      = &(x^2+5x+6)^2+2x(x^2+5x+6)+x^2 \\	
      = &(x^2+5x+6+x)^2\\
      = &(x^2+6x+6)^2
    \end{align*}
    ```
  
1. $(x^2+xy+y^2)^2-4xy(x^2+y^2)$
    ```{admonition} Answer
    \begin{align*}
      ~&(x^2+xy+y^2)^2-4xy(x^2+y^2)\\
      = &[(x^2+y^2)+xy]^2-4xy(x^2+y^2) \\
      = &(x^2+y^2)^2+2xy(x^2+y^2)+(xy)^2-4xy(x^2+y^2)\\
      = &(x^2+y^2)-2xy(x^2+y^2)+(xy)^2\\
      = &(x^2+y^2-xy)^2
    \end{align*}
    ```
  
1. $(x^2+3x+2)(4x^2+8x+3)-90$
    ```{admonition} Answer
    \begin{align*}
      ~&(x^2+3x+2)(4x^2+8x+3)-90 \\
      = &(x+1)(x+2)(2x+3)(2x+1)-90 \\
      = &(2x^2+5x+3)(2x^2+5x+2)-90 \\
      = &(2x^2+5x+2)^2 + (2x^2+5x+2) -90			\\
      = &(2x^2+5x+2+10)(2x^2+5x+2-9)			\\
      = &(2x^2+5x+12)(2x^2+5x-7)\\
      = &(2x^2+5x+12)(2x+7)(x-1)
    \end{align*}
    ```
  
1. $(a^2+1)^2+(a^2+5)^2-4(a^2+3)^2$
    ```{admonition} Answer
    \begin{align*}
      ~& (a^2+1)^2+(a^2+5)^2-4(a^2+3)^2 \\
      = &(a^2+1)^2+[(a^2+5)+2(a^2+3)][(a^2+5)-2(a^2+3)]			\\
      = &(a^2+1)^2+(3a^2+11)(-a^2-1)			\\ 
      = &(a^2+1)(a^2+1-3a^2-11)			\\
      = &(a^2+1)(-2a^2-10)			\\
      = &-2(a^2+1)(a^2+5)
    \end{align*}
    ```
:::

:::{exercise} Factorise the following expressions.

1. $x^3-9x+8$
    ```{admonition} Answer
    \begin{align*}
      ~& x^3-9x+8\\
      = &x^3-1-9x+9 \\
      = &(x^3-1)-9(x-1)\\
      = &(x-1)(x^2+x+1)-9(x-1)\\
      = &(x-1)(x^2+x-8)
    \end{align*}
    ```
  
1. $(x+1)^4+(x^2-1)^2+(x-1)^4$
    ```{admonition} Answer
    \begin{align*}
      ~& (x+1)^4 + (x^2-1)^2 + (x-1)^4 \\
      = &(x+1)^4+\left[(x+1)(x-1)\right]^2+(x-1)^4 \\
      = &(x+1)^4+2\left[(x+1)(x-1)\right]^2+(x-1)^4-\left[(x+1)(x-1)\right]^2 \\
      = &\left[(x+1)^2+(x-1)^2\right]^2-\left[(x+1)(x-1)\right]^2	\\
      = &(2x^2+2+x^2-1)(2x^2+2-x^2+1) \\
      = &(3x^2+1)(x^2+3)
    \end{align*}
    ```
  
1. $x^3+4x^2-7x+2$
    ```{admonition} Answer
    \begin{align*}
      ~& x^3+4x^2-7x+2 \\
      = &(x^3-1)+(4x^2-7x+3)\\
      = &(x-1)(x^2+x+1)+(4x-3)(x-1)	\\
      = & (x-1)(x^2+x+1+4x-3)\\
      = & (x-1)(x^2+5x-2)
    \end{align*}
    ```
  
1. $a^4+b^4+c^4-2a^2b^2-2a^2c^2-2b^2c^2$
    ```{admonition} Answer
    \begin{align*}
      ~& a^4+b^4+c^4-2a^2b^2-2a^2c^2-2b^2c^2\\
      = &(a^2-b^2-c^2)^2-4b^2c^2		\\
      = &(a^2-b^2-c^2+2bc)(a^2-b^2-c^2-2bc)	\\
      = &[a^2-(b-c)^2][a^2-(b+c)^2]			\\
      = &(a+b-c)(a-b+c)(a+b+c)(a-b-c)
    \end{align*}
    ```
  
1. $x^4-7x^2+1$
    ```{admonition} Answer
    \begin{align*}
      ~& x^4-7x^2+1 = &x^4+2x^2+1-9x^2\\
      = &(x^2+1)^2-(3x)^2 \\
      = &(x^2+1-3x)(x^2+1+3x)	\\
      = &(x^2+3x+1)(x^2-3x+1)
    \end{align*}
    ```
:::