(chap07-extraEx)=
# Challenging Exercise 7


%Q1
:::{exercise}
:label: chap07-extraEx-q1
  $y=f(x)$ is an even function and it is symmetric about the $y-$axis
($x=0$). Then the function $y=f(x-1)$ symmetric about:

1.  $x=0$ 
1.  $x=1$ 
1.  $x=-1$ 
1.  $x=2$

:::


 

%Q2
:::{exercise} 
:label: chap07-extraEx-q2

Supposing $0<a<1$ and $b<-1$, which quadrant the function
  $\displaystyle y=a^x+ b$ doesn't pass? 
  
1. first
1. second 
1. third 
1. fourth
:::  




%Q3
:::{exercise}
:label: chap07-extraEx-q3

 When the value of the function $y=\ln x + 2 x -6$ is zero, which
condition should $x$ satisfy?


- $1<x<2$
- $2<x<3$
- $3<x<4$
- $4<x<5$

:::




 %Q4
:::{exercise}
:label: chap07-extraEx-q4

The sum of the minimum and maximum of $\displaystyle y=a^x$ ($0\leq x  \leq 1$) is 3, then $a$ is: 


1.  0.5
1.  2
1.  4
1.  0.25

  
:::



  
  %Q5
:::{exercise}
:label: chap07-extraEx-q5

$f(x)$ is an odd function, when $x>0$, $f(x)=\log_2 x$; when $x<0$, $f(x)$ should be :
  
  
1.  $-\log_2 x$
1.  $\log_2 (-x)$
1.  $\log_2 x$
1.  $-\log_2 (-x)$     
:::





  %Q6
:::{exercise}
:label: chap07-extraEx-q6

 The real solutions of quadratic equation $2(m+1)x^2+4mx+3m-2=0$ 
  have the same sign, then $m$ should satisfy:
  

1.  $-2<m<-1$
1.  $-2\leq m < -1 $ or $ \dfrac{2}{3} < m \leq 1$       
1.  $m<-1$ or $ m> \dfrac{2}{3}$
1.  $-2<m<-1$ or $ \dfrac{2}{3}<m \leq 1$


:::



  %Q7
:::{exercise}
:label: chap07-extraEx-q7

 $f(x)$ is odd function and $f(x+2)=f(x)$, when $0<x<1$, $f(x)=\log_2
  x$. Supposing $\displaystyle a=f\left(\dfrac{6}{5}\right)$, $\displaystyle
  b=f\left(\dfrac{3}{2}\right)$, $\displaystyle c=f\left(\dfrac{5}{2}\right)$,
  then they have the following relationship:


1.  $a<b<c$
1.  $b<a<c$
1.  $c<b<a$
1.  $c<a<b$     
        


:::



  %Q8 
:::{exercise} 
:label: chap07-extraEx-q8

Supposing $0<x<y<a<1$, which of the followings is correct?
 

1.  $\log_a (xy)<0$
1.  $0<\log_a(xy)<1$
1.  $1<\log_a(xy)$
1.  $\log_a(xy)>2$    
:::



  %Q9 
:::{exercise}
:label: chap07-extraEx-q9

Supposing $f(x)=\log\dfrac{2+x}{2-x}$, the domain of
the $ g(x)=
f\left(\dfrac{x}{2}\right)+f\left(\dfrac{2}{x}\right)$ should be :


1.  $(-4, 0) \cup (0, 4)$
1.  $(-4, -1) \cup (1, 4)$        
1.  $(-2, -1) \cup (1, 2)$
1.  $(-4, -2) \cup (2, 4)$

:::

  %Q10
:::{exercise}
:label: chap07-extraEx-q10

$$
  f(x) = \left\{
    \begin{array}{ll}
      (3a-1)x+4a, & x<1 \\
      \log_a x, & x\geq 1
    \end{array}
    \right.
$$

is a decreasing function, the range of $a$ is:


1.  $0<a<1$
1.  $\displaystyle 0<a<\dfrac{1}{3}$
1.  $\displaystyle \dfrac{1}{7}\leq a < \dfrac{1}{3}$    
1.  $\displaystyle \dfrac{1}{7} \leq a < 1$


:::



  %Q11
:::{exercise} 
:label: chap07-extraEx-q11

The domain of the function $y=\log_a(kx^2+4kx+3)$ is $\mathbb{R}$, find the
ranges of $k$.
:::

:::{solution} chap07-extraEx-q11
:class: dropdown
For a general logarithm function $f(x)=\log_a x$, $x$ should be larger than zero.
So for $y=\log_a (kx^2+4kx+3)$, we can obtain

$$kx^2+4kx+3>0
$$
 for $x\in \mathbb{R}$. We need to find the minimum value
of $g(x)=kx^2+4kx+3$ and ensure it is larger than zero
\begin{align*}
  g(x)= & kx^2+4kx+3 \\
  = & kx^2+4kx+4k-4k+3 \\
  = & k(x^2+4x+4)-4k+3 \\
  = & k(x+2)^2 +3-4k
\end{align*}
When $x=-2$, the minimum of $g(x)$ is $3-4k$ and it should be larger than zero, so

$$3-4k>0
$$

therefore 

$$k< \dfrac{3}{4}
$$
    
:::


  %Q12
:::{exercise} 
:label: chap07-extraEx-q12

Function $f(x)=2ax+2a+1$, $x \in [-1, 1]$ has both positive and
negative values, find the ranges of $a$.
:::



  %Q13
:::{exercise}
:label: chap07-extraEx-q13

The brightness of light reduces by $10\%$ when the light passes
through a piece of glass of 1 cm thickness. How many pieces of glasses with
the same thickness would be needed to reduce the brightness of light by
$\dfrac{2}{3}$.

:::



  %Q14
:::{exercise}
:label: chap07-extraEx-q14

Supposing $a>0$, $\displaystyle f(x)= \dfrac{e^x}{a}+\dfrac{a}{e^x}$
is an even function.

1. Find the value of $a$;
2. Prove that $f(x)$ is an increasing function for $x\in (0, +\infty)$.
:::




  %Q15
:::{exercise} 
:label: chap07-extraEx-q15

Supposing the domain of the function $\displaystyle f(x) =
\sqrt{2-\dfrac{x+3}{x-1}}$ is $\mathbf{A}$, the domain of the function 
$g(x) = \log \left[(x-a-1)(2a-x)\right]$, $a<1$ is $\mathbf{B}$.

1. Find $\mathbf{A}$;
2. If $\mathbf{B} \subseteq \mathbf{A}$, find the ranges of $a$.
:::



  % Q16
:::{exercise} 
:label: chap07-extraEx-q16

Sketch the inverse function for each function in the following graphs.

1. 
    ```{figure} /images/07/Ex7Q16a.svg
    ---
    width: 400px
    name: figure-Ex7Q16a
    ---

2. 
    ```{figure} /images/07/Ex7Q16b.svg
    ---
    width: 400px
    name: figure-Ex7Q16b
    ---

:::



## Solutions to Challenging Exercise 7

:::{solution} chap07-extraEx-q1
:class: dropdown
Supposing $f(x)=x^2$, it is an even function and symmetric about $x=0$. We could obtain $f(x-1)=(x-1)^2$, it is symmetric about $x=1$ as shown in the following figure.

```{figure} /images/07/Ex7Q1.svg
---
width: 400px
name: figure-Ex7Q1
---
```
:::


:::{solution} chap07-extraEx-q2
:class: dropdown

Supposing $a=0.5$ and $b=-2$, We could have the following graph.
  
```{figure} /images/07/Ex7Q2.svg
---
width: 400px
name: figure-Ex7Q2
---
```

Apparently, the curve doesn't pass the first quadrant.

:::

:::{solution} chap07-extraEx-q3
:class: dropdown
When $y=\ln x + 2x -6=0$, we can obtain

$$\ln x = 6-2x$$

This will be equivalent to solve the following simultaneous equations

$$
  \begin{cases}
    y=\ln x \\
    y=6-2x
  \end{cases}
$$

Drawing these two functions, we obtain

```{figure} /images/07/Ex7Q3.svg
---
width: 400px
name: figure-Ex7Q3
---
```

  Apparently, the $x-$coordinate of the intersection is between 2 and 3.
:::

:::{solution} chap07-extraEx-q4
:class: dropdown
  $a^0+a^1=3$
  
  $1+a=3$
  
  $a=2$
:::

:::{solution} chap07-extraEx-q5
:class: dropdown
When $x>0$, we have $x=|x|$ and $f(x)=f(|x|)=\log_2 |x|$. 

Since $f(x)$ is odd, so we have $f(-|x|)=-f(|x|)$ when $x>0$. 

Therefore, when $x<0$  we should have 

$$f(x)=-f(|x|) = -\log_2 |x| = -\log_2 (-x) 
$$

:::

:::{solution} chap07-extraEx-q6
:class: dropdown
The quadratic equation has real solutions, so its discriminator should
be larger than or equal to zero
\begin{align*}
  \Delta & = b^2-4ac  \\
          & = (4m)^2 - 4\left[2(m+1)\right](3m-2) \\
          & = 16m^2 - 8(m+1)(3m-2) \\
          & = 16m^2 - 8(3m^2+m-2) \\
          & = 8\left[ 2m^2 -(3m^2+m-2)\right] \\
          & = 8(-m^2-m+2) \\
          & = -8(m^2+m-2) \\
          & = -8(m+2)(m-1)
\end{align*}
$\Delta \geq 0$, so $ -8(m+2)(m-1)\geq 0 $. Therefore we obtain

$$-2 \leq m \leq 1
$$


The product of the two solutions is given by

$$x_1 x_2 = \dfrac{c}{a} = \dfrac{3m-2}{2(m+1)}
$$

The two solutions of the equation have the same sign, so 

$$\dfrac{3m-2}{2(m+1)} \geq 0 
$$

Therefore we can obtain
$m<-1$ or $m\geq \dfrac{2}{3}$

In conclusion, $m$ should satisfy the condition

$$-2\leq m<-1
$$
 or

$$\dfrac{2}{3}\leq m \leq 1 
$$

:::


:::{solution} chap07-extraEx-q7
:class: dropdown
When $0<x<1$, $f(x)=\log_2 x$ and it is an odd function, so we have the following graph

```{figure} /images/07/Ex7Q7.svg
---
width: 400px
name: figure-Ex7Q7
---
```

where $f(-x)=-f(x)$ for $-1\leq x <0 $ and $ 0< x \leq 1$.


We also know that the function is periodic, and its period is 2. So we can obtain
\begin{align*}
  & a = f\left( \dfrac{6}{5}\right)= f\left( 2- \dfrac{4}{5}\right) = f\left( -\dfrac{4}{5}\right)= -f\left( \dfrac{4}{5}\right) \\
  & b = f\left( \dfrac{3}{2}\right)= f\left( 2- \dfrac{1}{2}\right) = f\left( -\dfrac{1}{2}\right)= -f\left( \dfrac{1}{2}\right) \\
  & c = f\left( \dfrac{5}{2}\right)= f\left( 2+ \dfrac{1}{2}\right) = f\left(  \dfrac{1}{2}\right)=  f\left( \dfrac{1}{2}\right)  
\end{align*}
Marking these points on the graph, we will know that $c < a < b$.
:::

:::{solution} chap07-extraEx-q8
:class: dropdown
Assuming $a^m = x$ and $a^n=y$, we could obtain that

$$m>1, \quad n>1 
$$

So
\begin{align*}
  & \log_a x = m > 1 \\
  & \log_a y = n > 1
\end{align*}
Therefore $\log_a x + \log_a y = \log_a (xy) = m+n>2 $
:::


:::{solution} chap07-extraEx-q9
:class: dropdown
\begin{align*}
  g(x) & = f(\dfrac{x}{2}) + f(\dfrac{2}{x}) \\
        & = \log \dfrac{2+\dfrac{x}{2}}{2- \dfrac{x}{2}} + \log \dfrac{2+\dfrac{2}{x}}{2-\dfrac{2}{x}} \\
        & = \log \dfrac{4+x}{4-x} + \log \dfrac{x+1}{x-1}  \qquad(x\neq 0) \\
\end{align*}
For a logarithm function $\log X$, $X$ should be larger than zero, therefore we should have

$$
\left\{
    \begin{aligned}
      & \dfrac{4+x}{4-x} > 0   \qquad(1)\\
      & \dfrac{x+1}{x-1}> 0    \qquad(2)
    \end{aligned}
  \right .
$$

From condition (1), we obtain $x\in (-4, 4)$.  From condition (2), we obtain
$x\in (-\infty, -1) \cup (1,+\infty)$. $x$ should satisfy both conditions, therefore we obtain

$$x \in (-4, -1) \cup (1, 4)
$$

:::


:::{solution} chap07-extraEx-q10
:class: dropdown
$f(x)$ is a decreasing function, therefore we can know that

1. $(3a-1)x+4a$  is decreasing for $x<1$
2. $\log_a x$ is decreasing for $x\ge 1$
3. $\left.\left[ (3a-1)x+4a\right]\right|_{x=1} \ge \left. \log_a x \right|_{x=1}$


From the first condition, we know that the function is a straight line for
$x<1$ and it should have a negative gradient, therefore

$$3a-1 <0  \Rightarrow a<\dfrac{1}{3}
$$


From the second condition, we know that $a$ should be a positive number less
than 1, therefore

$$0<a<1
$$


From the third condition, we obtain

$$(3a-1)+4a \ge \log_a 1
$$


$$\Rightarrow 7a-1 \ge 0
$$


$$a \ge \dfrac{1}{7}
$$


All the three conditions should be satisfied, therefore

$$\dfrac{1}{7} \le a < \dfrac{1}{3}
$$

:::


:::{solution} chap07-extraEx-q12
:class: dropdown
This is a straight line segment, at the two ends the function has the two
extrema (maximum and minimum).
\begin{align*}
  & f(-1)=2a(-1)+2a+1=1 > 0 \\
  & f(1)=2a(1)+2a+1=4a+1
\end{align*}
As the function also has negative values, we can obtain 

$$f(1)=4a+1< 0
$$


$$\Rightarrow a < -\dfrac{1}{4}
$$

:::


:::{solution} chap07-extraEx-q13
:class: dropdown
Without any glass, the brightness is 100\%. After one piece of glass, the
brightness becomes $100\% \times 0.9^1$.  After $x$ pieces of glass, the
brightness is

$$b(x) = 100\% \times 0.9^x
$$

Reducing the brightness by $\dfrac{2}{3}$, we can obtain

$$100\% \times 0.9^x = \dfrac{1}{3}
$$

Therefore

$$x= \log_{0.9} \dfrac{1}{3} = 10.43
$$

Thus we need 11 pieces of glasses.
:::


:::{solution} chap07-extraEx-q14
:class: dropdown
1.       
    $$f(x)= \dfrac{e^x}{a}+\dfrac{a}{e^x} = \dfrac{1}{a} e^x + a e^{-x}
    $$
          
    $$f(-x)= \dfrac{e^{-x}}{a}+\dfrac{a}{e^{-x}} = \dfrac{1}{a} e^{-x} + a e^x
    $$

    $f(x)$ is even, so $f(-x)=f(x)$, we can obtain
          
    $$\dfrac{1}{a} e^x + a e^{-x} = \dfrac{1}{a} e^{-x} + a e^x 
    $$

          
    $$\Rightarrow \left(\dfrac{1}{a}-a\right)e^x + \left(a-\dfrac{1}{a}\right)e^{-x} = 0
    $$

    Since $e^x > 0$ and $e^{-x}>0$ for $x\in R$, we can obtain
          
    $$\dfrac{1}{a}-a =0 
    $$

          
    $$\Rightarrow a=\pm 1
    $$

    $a>0$, so $a=1$.

2. 
    Idea: $x\in (0, +\infty)$, for $u>0$ if we could prove $\Delta = f(x+u) - f(x)>0$, then
    $f(x)$ is an increasing function.
    \begin{align*}
      \Delta & = f(x+u) - f(x) \\
              & = \left ( e^{x+u} + e^{-x-u}\right) - \left( e^x + e^{-x} \right) \\
              & = \left ( e^{x+u} - e^{x}\right) + \left( e^{-x-u} - e^{-x} \right) \\
              & = e^x \left(e^u-1\right) + e^{-x} ( e^{-u} -1) \\
              & = e^x \left(e^u-1\right) - e^{-x} ( 1-e^{-u} ) \\
              & = e^{-x}\left(1-e^{-u}\right) \left[ \dfrac{e^x(e^u-1)}{e^{-x}(1-e^{-u})} - 1 \right] \\
              & = e^{-x}\left(1-e^{-u}\right) \left[ \dfrac{e^{2x}(e^u-1)}{(1-e^{-u})} - 1 \right] \\
              & = e^{-x}\left(1-e^{-u}\right) \left[ \dfrac{e^{2x}e^u(e^u-1)}{e^u(1-e^{-u})} - 1 \right] \\
              & = e^{-x}\left(1-e^{-u}\right) \left[ \dfrac{e^{2x}e^u(e^u-1)}{e^u-1} - 1 \right] \\
              & = e^{-x}\left(1-e^{-u}\right) \left( e^{2x}e^u - 1 \right) \\
    \end{align*}
    For $x>0$ and $u>0$, we know

    - $e^x>1$, $e^{2x}>1$ and $e^u>1$  $\quad \Rightarrow e^{2x}e^u - 1> 0$
    - $0<e^{-x}<0$
    - $0<e^{-u}<1$ $\quad \Rightarrow 0<1-e^{-u}<1 $ 

    Thus $e^{-x}\left(1-e^{-u}\right) \left( e^{2x}e^u - 1 \right)>0$, and we
    have proved $f(x)$ is an increasing function for $x\in (0, +\infty)$.
:::


:::{solution} chap07-extraEx-q15
:class: dropdown
1.
    Under the square bracket, the value should satisfy two conditions

    - $\displaystyle 2-\dfrac{x+3}{x-1} \ge 0$
    - $x-1\ne 0$

    From the first condition, we obtain
    \begin{align*}
                  & 2-\dfrac{x+3}{x-1} \ge 0 \\
      \Rightarrow &  \dfrac{x-5}{x-1} \ge 0  \\
      \Rightarrow & x\ge 5 ~~ \mathrm{or}~~ x \le 1
    \end{align*}
    From the second condition, we obtain

    $$x \ne 1
    $$

    Thus $x\ge 5$ or $x < 1$, therefore
    $\mathbf{A}=(-\infty, 1) \cup [5,+\infty)$

2.
    For $g(x)=\log \left[(x-a-1)(2a-x)\right]$, $a<1$, we should have
    
    $$\quad (x-a-1)(2a-x)>0
    $$

    
    $$\Rightarrow (x-a-1)(x-2a)<0 
    $$

    
    $$\Rightarrow 2a < x < a+1 
    $$


    $$\mathbf{B}=(2a, a+1) 
    $$

    Note: $a<1$, ~~$2a<a+1$

    As $\mathbf{B} \subseteq \mathbf{A}$, we could have

    $$a+1 \le 1   \Rightarrow a\le 0
    $$

    or 

    $$2a \ge 5    \Rightarrow a\ge \dfrac{5}{2}   
    $$

    Because $a<1$, so we should have $a\le 0$ to ensure $\mathbf{B}$ is a subset of $\mathbf{A}$.
:::

:::{solution} chap07-extraEx-q16
:class: dropdown
A function and its inverse are symmetric about the straight line $y=x$.

1. 
    ```{figure} /images/07/Ex7Q16aSol.svg
    ---
    width: 400px
    name: figure-Ex7Q16aSol
    ---

2. 
    ```{figure} /images/07/Ex7Q16bSol.svg
    ---
    width: 400px
    name: figure-Ex7Q16bSol
    ---

:::